started with proof rules

ex_lang.thy
@@ -38,21 +38,21 @@ datatype expr =
 
 datatype stmt =
     Assert expr
+  | Assume expr
   | Assign var expr
-  | If expr expr stmt stmt
+  | If expr stmt stmt
   | While expr stmt
-  | Seq expr expr
+  | Seq stmt stmt
 
 
 subsection \<open>Semantics\<close>
 
-text \<open>We now define the semantics of the language using a big step operational semantics.\<close>
+text \<open>We now define the semantics of the language using a small step operational semantics.\<close>
 
 
 
 record state =
   varState :: "var \<rightharpoonup> val"
-  error :: "bool"
 
 
 value "Some (5::int) \<bind> (\<lambda>x. Some (x +  1))"
@@ -85,17 +85,173 @@ fun eval :: "state \<Rightarrow> expr \<rightharpoonup> val" where
 | "eval S (VarRead v) = varState S v"
 | "eval S (Const v) = Some v"
 
-definition "withError S \<equiv> S\<lparr>error := True\<rparr>"
 
 definition "updateVar S x v \<equiv> S\<lparr>varState := (varState S)(x \<mapsto> v)\<rparr>" 
 
-inductive step :: "state \<Rightarrow> stmt \<Rightarrow> state \<Rightarrow> bool" where
-assert_true: 
-"eval S e = Some (BoolVal True) \<Longrightarrow> step S (Assert e) S"
-| assert_false:
-"eval S e \<noteq> Some (BoolVal True) \<Longrightarrow> step S (Assert e) (withError S)"
-| assign:
-"eval S e = Some v \<Longrightarrow> step S (Assign x e) (updateVar S x v)" 
+datatype step_res = Final state | NonFinal state stmt | Error | Invalid
+
+fun step :: "state \<Rightarrow> stmt \<Rightarrow> step_res" where
+  "step S (Assert e) = (case eval S e of Some (BoolVal True) \<Rightarrow> Final S | _ \<Rightarrow> Error)"
+| "step S (Assume e) = (case eval S e of Some (BoolVal True) \<Rightarrow> Final S | _ \<Rightarrow> Invalid)"
+| "step S (Assign x e) = (case eval S e of Some v \<Rightarrow> Final (updateVar S x v) | _ \<Rightarrow> Error)"
+| "step S (If c t f) = (case eval S c of Some (BoolVal True) \<Rightarrow> NonFinal S t
+                                       | Some (BoolVal False) \<Rightarrow> NonFinal S f 
+                                       | _ \<Rightarrow> Error)"
+| "step S (While c b) = (case eval S c of Some (BoolVal True) \<Rightarrow> NonFinal S (Seq b (While c b))
+                                       | Some (BoolVal False) \<Rightarrow> Final S 
+                                       | _ \<Rightarrow> Error)"
+| "step S (Seq a b) = (case step S a of Final S' \<Rightarrow> NonFinal S' b
+                                      | NonFinal S' a' \<Rightarrow> NonFinal S' (Seq a' b) 
+                                      | Error \<Rightarrow> Error 
+                                      | Invalid \<Rightarrow> Invalid)"
+
+
+inductive steps :: "state \<Rightarrow> stmt \<Rightarrow> state option \<Rightarrow> bool" where
+  final: "step S stmt = Final S' \<Longrightarrow>  steps S stmt (Some S')"
+| nonfinal: "\<lbrakk>step S stmt = NonFinal S' stmt'; steps S' stmt' S''\<rbrakk> \<Longrightarrow> steps S stmt S''"
+| error: "step S stmt = Error \<Longrightarrow> steps S stmt None"
+
+
+text "We also show some big step forms of the rules:"
+
+lemma steps_big_seq1:
+  assumes "steps S a S1"
+    and "S1 = Some S'"
+    and "steps S' b S''"
+  shows "steps S (Seq a b) S''"
+  using assms proof (induct rule: steps.induct)
+case (final S stmt S')
+  then show ?case
+    using nonfinal by auto
+next
+  case (nonfinal S stmt S' stmt' S'')
+  then show?case 
+    by (metis step.simps(6) step_res.simps(16) steps.simps)
+next
+  case (error S stmt)
+  then show ?case 
+    by blast
+qed
+
+lemma steps_big_seq:
+  assumes "steps S a (Some S')"
+    and "steps S' b S''"
+  shows "steps S (Seq a b) S''"
+  using assms(1) assms(2) steps_big_seq1 by auto
+
+lemma steps_big_seq_None1:
+  assumes "steps S a S'"
+    and "S' = None"
+  shows "steps S (Seq a b) None"
+  using assms proof (induct rule: steps.induct)
+  case (final S stmt S')
+  then show ?case 
+    by auto
+next
+  case (nonfinal S stmt S' stmt' S'')
+  then show ?case
+    by (simp add: steps.nonfinal)
+next
+  case (error S stmt)
+  then show ?case 
+    using steps.error by auto
+qed
+
+
+lemma steps_big_seq_None:
+  assumes "steps S a None"
+  shows "steps S (Seq a b) None"
+  using assms steps_big_seq_None1 by auto
+
+lemma step_seq:
+  assumes "step S (Seq a b) = Final S'"
+  shows "step S a = Final S'"
+  using assms by (auto split: step_res.splits)
+
+
+lemma steps_big_seq_iff:
+  shows "steps S (Seq a b) S'' \<longleftrightarrow> (steps S a None \<and> S'' = None \<or> (\<exists>S'. steps S a (Some S') \<and> steps S' b S''))"
+proof (rule iffI conjI; (elim disjE conjE exE)?)
+  assume a0: "steps S a None"
+    and a1: "S'' = None"
+
+  show "steps S (Seq a b) S''"
+    by (simp add: a0 a1 steps_big_seq_None)
+next
+  fix S'
+  assume a0: "steps S a (Some S')"
+    and a1: "steps S' b S''"
+
+  show "steps S (Seq a b) S''"
+    using a0 a1 steps_big_seq1 by blast
+next
+  assume a0: "steps S (Seq a b) S''"
+
+  define stmt where "stmt \<equiv> Seq a b"
+
+  have "steps S stmt S''"
+    by (simp add: a0 stmt_def)
+
+  from `steps S stmt S''` stmt_def
+  have "\<exists>S'. steps S a S' \<and> (case S' of Some S' \<Rightarrow> steps S' b S'' | None \<Rightarrow> S'' = None)"
+  proof (induct  arbitrary: a rule: steps.induct)
+    case (final S S')
+    then show ?case 
+      using step_seq by force
+  next
+    case (nonfinal S S' stmt' S'')
+
+    from `step S (Seq a b) = NonFinal S' stmt'`
+    show ?case
+      apply (auto split: step_res.splits)
+      using final nonfinal.hyps(2) apply fastforce
+      using nonfinal.hyps(3) steps.nonfinal by blast
+  next
+    case (error S)
+    then show ?case 
+      apply (auto split: step_res.splits)
+      using steps.error by fastforce
+  qed
+
+
+  from this
+  obtain S' where "steps S a S'"
+    and "case S' of Some S' \<Rightarrow> steps S' b S'' | None \<Rightarrow> S'' = None"
+    by blast
+
+  from this
+  show "steps S a None \<and> S'' = None \<or> (\<exists>S'. steps S a (Some S') \<and> steps S' b S'')"
+    using case_optionE by blast
+qed
+   
+                              
+
+lemma steps_big_if_True:
+  assumes "eval S c = Some (BoolVal True)"
+    and "steps S t S'"
+  shows "steps S (If c t f) S'"
+  using assms nonfinal steps_big_seq1 by auto
+
+lemma steps_big_if_False:
+  assumes "eval S c = Some (BoolVal False)"
+    and "steps S f S'"
+  shows "steps S (If c t f) S'"
+  using assms nonfinal steps_big_seq1 by auto
+
+
+lemma steps_big_while_True:
+  assumes "eval S c = Some (BoolVal True)"
+    and "steps S b (Some S')"
+    and "steps S' (While c b) S''"
+  shows "steps S (While c b) S''"
+  using assms nonfinal steps_big_seq1 by auto
+
+lemma steps_big_while_False:
+  assumes "eval S c = Some (BoolVal False)"
+  shows "steps S (While c b) (Some S)"
+  by (simp add: assms final)
+
+
 
 
 end
